\documentclass{article}
\usepackage{amsmath}

\title{Confidence distribution for exact permutation method}
\author{Travis Andersen}

\begin{document}
\maketitle  

Let $\theta \in \Theta$ and $\textbf{Z} \in \mathcal{Z}$. A confidence distribution is a function $C(\theta|\textbf{Z})$ on $\Theta \times \mathcal{Z} \to [0, 1]$ that satisfies the following:

\begin{align*}
  C(\theta|\textbf{z}) = P_\theta(t(z) \geq t(z_{obs})) = \frac
  {\sum_{u^*=t(z_{obs})}^{\text{max}(t(z))} C(u^*|s^\alpha(z), s^\delta(z), s^{\delta_2}(z))e^{\theta u^*}}
  {\sum_{u=\text{min}(t(z))}^{\text{max}(t(z))} C(u|s^\alpha(z), s^{\delta_1}(z), s^{\delta_2}(z))e^{\theta u}}
  = \alpha
\end{align*}

\begin{enumerate}
  \item For each $\textbf{Z} \in \mathcal{Z}$, $C(\theta|\textbf{z})$ is a cdf for $\theta$. 
  \item When $\theta$ is the true parameter, $C(\theta|\textbf{z}) \sim U(0, 1)$
\end{enumerate}

\section{Show $C(\theta|\textbf{z})$ is a cdf}
\subsection{Show $\lim_{\theta \to -\infty} C(\theta|\textbf{z}) = 0$ and $\lim_{\theta \to \infty} C(\theta|\textbf{z}) = 1$}
\begin{align*}
  \lim_{\theta \to -\infty} C(\theta|\textbf{z}) 
  &= \lim_{\theta \to -\infty} \frac
  {\sum_{u^*=t(z_{obs})}^{\text{max}(t(z))} C(u^*|s^\alpha(z), s^\delta(z), s^{\delta_2}(z))e^{\theta u^*}}
  {\sum_{u=\text{min}(t(z))}^{\text{max}(t(z))} C(u|s^\alpha(z), s^{\delta_1}(z), s^{\delta_2}(z))e^{\theta u}} \\
  &= \lim_{\theta \to -\infty} \frac
  {\sum_{u^*=t(z_{obs})-\text{min}(t(z))}^{\text{max}(t(z))-\text{min}(t(z))} 
  C(u^*+\text{min}(t(z))|s^\alpha(z), s^\delta(z), s^{\delta_2}(z))e^{\theta (u^*+\text{min}(t(z)))}}
  {\sum_{u=0}^{\text{max}(t(z))-\text{min}(t(z))} 
  C(u+\text{min}(t(z))|s^\alpha(z), s^{\delta_1}(z), s^{\delta_2}(z))e^{\theta (u+\text{min}(t(z)))}} \\
  &= \lim_{\theta \to -\infty} \frac
  {e^{\theta \text{min}(t(z))} \sum_{u^*=t(z_{obs})-\text{min}(t(z))}^{\text{max}(t(z))-\text{min}(t(z))} 
  C(u^*+\text{min}(t(z))|s^\alpha(z), s^\delta(z), s^{\delta_2}(z))e^{\theta u^*}}
  {e^{\theta \text{min}(t(z))} \sum_{u=0}^{\text{max}(t(z))-\text{min}(t(z))} 
  C(u+\text{min}(t(z))|s^\alpha(z), s^{\delta_1}(z), s^{\delta_2}(z))e^{\theta u}} \\
  &= \lim_{\theta \to -\infty} \frac
  {\sum_{u^*=t(z_{obs})-\text{min}(t(z))}^{\text{max}(t(z))-\text{min}(t(z))} 
  C(u^*+\text{min}(t(z))|s^\alpha(z), s^\delta(z), s^{\delta_2}(z))e^{\theta u^*}}
  {C(\text{min}(t(z))|s^\alpha(z), s^{\delta_1}(z), s^{\delta_2}(z))+\sum_{u=1}^{\text{max}(t(z))-\text{min}(t(z))} 
  C(u+\text{min}(t(z))|s^\alpha(z), s^{\delta_1}(z), s^{\delta_2}(z))e^{\theta u}} \\
  &= \frac{0}{C(\text{min}(t(z))|s^\alpha(z), s^{\delta_1}(z), s^{\delta_2}(z))+0} = 0
  \text{, for } t(z_{obs}) > \text{min}(t(z)) \\
\end{align*}

\begin{align*}
  \lim_{\theta \to \infty} C(\theta|\textbf{z}) 
  &= \lim_{\theta \to \infty} \frac
  {\sum_{u^*=t(z_{obs})}^{\text{max}(t(z))} C(u^*|s^\alpha(z), s^\delta(z), s^{\delta_2}(z))e^{\theta u^*}}
  {\sum_{u=\text{min}(t(z))}^{\text{max}(t(z))} C(u|s^\alpha(z), s^{\delta_1}(z), s^{\delta_2}(z))e^{\theta u}} \\
  &= \lim_{\theta \to \infty} \frac
  {e^{-\theta \text{max}(t(z))} \sum_{u^*=t(z_{obs})}^{\text{max}(t(z))} 
  C(u^*|s^\alpha(z), s^\delta(z), s^{\delta_2}(z))e^{\theta u^*}}
  {e^{-\theta \text{max}(t(z))} \sum_{u=\text{min}(t(z))}^{\text{max}(t(z))} 
  C(u|s^\alpha(z), s^{\delta_1}(z), s^{\delta_2}(z))e^{\theta u}} \\
  &= \lim_{\theta \to \infty} \frac
  {\sum_{u^*=t(z_{obs})}^{\text{max}(t(z))} 
  C(u^*|s^\alpha(z), s^\delta(z), s^{\delta_2}(z))e^{\theta (u^*-\text{max}(t(z)))}}
  {\sum_{u=\text{min}(t(z))}^{\text{max}(t(z))} 
  C(u|s^\alpha(z), s^{\delta_1}(z), s^{\delta_2}(z))e^{\theta (u^*-\text{max}(t(z)))}} \\
  &= \lim_{\theta \to \infty} \frac
  {C(\text{max}(t(z)))|s^\alpha(z), s^\delta(z), s^{\delta_2}(z)) + \sum_{u^*=t(z_{obs})}^{\text{max}(t(z))-1} 
  C(u^*|s^\alpha(z), s^\delta(z), s^{\delta_2}(z))e^{\theta (u^*-\text{max}(t(z)))}}
  {C(\text{max}(t(z)))|s^\alpha(z), s^\delta(z), s^{\delta_2}(z)) + \sum_{u=\text{min}(t(z))}^{\text{max}(t(z))-1} 
  C(u|s^\alpha(z), s^{\delta_1}(z), s^{\delta_2}(z))e^{\theta (u^*-\text{max}(t(z)))}} \\
  &= \frac
  {C(\text{max}(t(z)))|s^\alpha(z), s^\delta(z), s^{\delta_2}(z)) + 0}
  {C(\text{max}(t(z)))|s^\alpha(z), s^\delta(z), s^{\delta_2}(z)) + 0} = 1 \\
\end{align*}

\subsection{Show $C(\theta|\textbf{z})$ is nondecreasing}

\begin{itemize}
  \item If a function has an inverse, it is bijective.
  \item If a function is increasing, then its inverse is increasing
  \item Therefore, we only need show that $R(\theta)$ is increasing to show that $R^{-1}(\theta)$ is increasing. 
\end{itemize}

\begin{align*}
  \text{log}[C(\theta|\textbf{z})] &= 
  \text{log}\left(
    \sum_{u^*=t(z_{obs})}^{\text{max}(t(z))} C(u^*|\cdot)e^{\theta u^*} 
  \right) - 
  \text{log}\left(
    \sum_{u=\text{min}(t(z))}^{\text{max}(t(z))} C(u|\cdot)e^{\theta u}
  \right) \\
  \frac{\partial}{\partial \theta} \text{log}[C(\theta|\textbf{z})] &= 
  \frac
  {\sum_{u^*=t(z_{obs})}^{\text{max}(t(z))} u^* C(u^*|\cdot)e^{\theta u^*}}
  {\sum_{u^*=t(z_{obs})}^{\text{max}(t(z))} C(u^*|\cdot)e^{\theta u^*}} -
  \frac
  {\sum_{u=\text{min}(t(z))}^{\text{max}(t(z))} u C(u|\cdot)e^{\theta u}}
  {\sum_{u=\text{min}(t(z))}^{\text{max}(t(z))} C(u|\cdot)e^{\theta u}} \\
  &= 
  \frac
  {\sum_{u^*=t(z_{obs})}^{\text{max}(t(z))} u^* C(u^*|\cdot)e^{\theta u^*}}
  {\sum_{u^*=t(z_{obs})}^{\text{max}(t(z))} C(u^*|\cdot)e^{\theta u^*}} -
  \frac
  {\sum_{u=\text{min}(t(z))}^{t(z_{obs})-1} u C(u|\cdot)e^{\theta u} + 
  \sum_{u^*=t(z_{obs})}^{\text{max}(t(z))} u^* C(u^*|\cdot)e^{\theta u^*}}
  {\sum_{u=\text{min}(t(z))}^{t(z_{obs})-1} C(u|\cdot)e^{\theta u} + 
  \sum_{u^*=t(z_{obs})}^{\text{max}(t(z))} C(u^*|\cdot)e^{\theta u^*}} \\
\end{align*}

\subsection{Show $C(\theta|\textbf{z})$ is right-continuous}
$C(\theta|\textbf{z})$ is a continuous function. 

\section{Show $C(\theta|\textbf{z}) \sim U(0, 1)$ when $\theta$ is the true parameter}
Combining information from independent sources through confidence distributions
pgs. 2-3

\end{document}